Add [dll_insert_before]

ind/DListLowInd.fst
@@ -1667,5 +1667,26 @@ let dll_insert_after (#t:Type) (d:dll t) (e:gpointer (node t)) (n:gpointer (node
     y
   )
 
+#reset-options
+
+let dll_insert_before (#t:Type) (d:dll t) (e:gpointer (node t)) (n:gpointer (node t)) :
+  StackInline (dll t)
+    (requires (fun h0 ->
+         (dll_valid h0 d) /\
+         (e `memP` reveal d.nodes) /\
+         (h0 `contains` n) /\
+         (node_not_in_dll h0 n d)))
+    (ensures (fun h0 y h1 ->
+         (* TODO: Write about what is modified *)
+         dll_valid h1 y)) =
+  let h0 = ST.get () in
+  extract_nodelist_contained h0 (reveal d.nodes) (reveal d.nodes `index_of` e);
+  let e1 = (!e).blink in
+  if is_null e1 then (
+    dll_insert_at_head d n
+  ) else (
+    extract_nodelist_conn h0 (reveal d.nodes) (reveal d.nodes `index_of` e - 1);
+    dll_insert_after d e1 n
+  )
 
 (* TODO *)
